src/spec/TLS13.Wire.Spec.RevealDecode.fst
@@ -8,6 +8,8 @@ module T = TLS13.Types
 module Seq = FStar.Seq
 module U8 = FStar.UInt8
 module WS = TLS13.Wire.Spec
+module GHS = TLS13.Wire.Generated.Handshake
+module LP = LowParse.Spec
 
 let lemma_parse_record_from_header raw =
   let flen = U8.v (Seq.index raw 3) * 256 + U8.v (Seq.index raw 4) in
@@ -45,3 +47,22 @@ let lemma_parse_tls_message_change_cipher_spec fragment =
   WS.lemma_byte_v 1;
   assert (U8.v (Seq.index ccs 0) == 1);
   Seq.lemma_eq_intro fragment ccs
+
+let lemma_parse_tls_message_no_client_hello ct fragment ch =
+  match ct with
+  | T.Handshake ->
+    (match LP.parse GHS.handshake_parser fragment with
+     | None -> ()
+     | Some (h, _) ->
+       match h with
+       | GHS.Body_client_hello _ -> ()
+       | GHS.Body_server_hello _ -> ()
+       | GHS.Body_encrypted_extensions _ -> ()
+       | GHS.Body_certificate _ -> ()
+       | GHS.Body_certificate_verify _ -> ()
+       | GHS.Body_finished _ -> ()
+       | GHS.Body_key_update _ -> ()
+       | GHS.Body_new_session_ticket _ -> ())
+  | T.ApplicationData -> ()
+  | T.Alert -> ()
+  | T.ChangeCipherSpec -> ()
